@prefix : <http://example.org/organization#>.
@prefix sh: <http://www.w3.org/ns/shacl#>.
@prefix rdf: <http://www.w3.org/1999/02/22-rdf-syntax-ns#>.
@prefix rdfs: <http://www.w3.org/2001/XMLSchema#>.
@prefix xsd: <http://www.w3.org/2000/01/rdf-schema#>.
@prefix id: <http://example.org/id#>.
@prefix pid: <http://example.org/pid#>.
@prefix foaf: <http://xmlns.com/foaf/0.1#>.
@prefix org: <http://www.w3.org/ns/org#>.
@prefix time: <http://www.w3.org/2006/time#>.


:BankCorporateTitle a rdfs:Class;
    rdfs:subClassOf org:Role;
    rdfs:label "Corporate Title"@en;
    rdfs:comment """A corporate title is a role defined by a banking organization that reflects both seniority, but also implies a certain 
                    salary band.  This is in contrast to other types of organization where corporate title and level (pay) are separate."""@en.

:StaffTitle a :BankCorporateTitle;
    rdfs:label "Staff"@en;
    rdfs:comment "A staff title is a corporate title that is held by a bank employee."@en.
:AVPTitle a :BankCorporateTitle;
    rdfs:label "AVP"@en;
    rdfs:comment "An AVP title is Assistant Vice President corporate title that is held by a bank employee."@en.
:VPTitle a :BankCorporateTitle;
    rdfs:label "VP"@en;
    rdfs:comment "A VP title is a Vice President corporate title that is held by a bank employee."@en.
:SVPTitle a :BankCorporateTitle;
    rdfs:label "Senior VP"@en;
    rdfs:comment "An VP title is a Senior Vice President corporate title that is held by a bank employee."@en.
:DIRTitle a :BankCorporateTitle;
    rdfs:label "Director"@en;
    rdfs:comment "A director title is a corporate title that is held by a bank employee."@en.
:SDIRTitle a :BankCorporateTitle;
    rdfs:label "Senior Director"@en;
    rdfs:comment "A SDIR title is a Senior Director corporate title that is held by a bank employee."@en.
:MDRTitle a :BankCorporateTitle;
    rdfs:label "Managing Director"@en;
    rdfs:comment "A managing director title is a corporate title that is held by a bank employee."@en.


:BankEmployee a rdfs:Class;
    rdfs:subClassOf foaf:Person;
    rdfs:label "Bank Employee"@en;
    rdfs:comment """A Bank Employee is a foaf:person who works for a bank, but will also have other properties
                    relating to the Bank such as an employee identifier, a corporate title, and organization."""@en.

:bankemployeesystem-id a rdf:Property;
    rdfs:domain :BankEmployee;
    rdfs:range id:id;
    rdfs:label "Employee ID"@en;
    rdfs:comment "An employee ID is a unique identifier for a bank employee."@en.

:bankemployeesystem-id a rdf:Property;
    rdfs:domain :BankEmployee;
    rdfs:range pid:pid;
    rdfs:label "Employee ID"@en;
    rdfs:comment "An employee ID is a unique identifier for a bank employee."@en.

:BankEmployeeShape a sh:NodeShape;
    sh:targetClass :BankEmployee;
    sh:nodeKind sh:IRI;
    sh:property [
        sh:path id:id;
        sh:datatype rdfs:string;
        sh:minCount 1;
        sh:maxCount 1;
        sh:minLength 7;
        sh:maxLength 7;
    ];
    sh:property [
        sh:path pid:pid;
        sh:datatype rdfs:string;
        sh:minCount 1;
        sh:maxCount 1;
        sh:minLength 7;
        sh:maxLength 7;
    ];
    sh:property [
        sh:path foaf:firstName;
        sh:datatype rdfs:string;
        sh:minCount 1;
        sh:maxCount 1;
        sh:minLength 1;
    ];
    sh:property [
        sh:path foaf:surname;
        sh:datatype rdfs:string;
        sh:minCount 1;
        sh:maxCount 1;
        sh:minLength 1;
    ].



############################################################################################################
#
# Bank Employee's Corporate Title for defined period of time
#
############################################################################################################
:BankEmployeeCorporateTitleMembership a rdfs:Class, sh:NodeShape;
    rdfs:subClassOf org:membership;
    sh:targetClass :BankEmployeeCorporateTitleMembership;
    sh:nodeKind sh:IRI;
    sh:property [
        sh:path org:member;
        sh:class :BankEmployee;
        sh:minCount 1;
        sh:maxCount 1;
    ];
    sh:property [
        sh:path :BankCorporateTitle;
        sh:node :BankCorporateTitle;
        sh:minCount 1;
        sh:maxCount 1;
        sh:in (:StaffTitle :AVPTitle :VPTitle :SVPTitle :DIRTitle :SDIRTitle :MDRTitle);
    ];
    sh:property [
        sh:path org:memberDuring;
        sh:class :BankEmployeeCorporateTitleMembershipDuration;
        sh:minCount 1;
        sh:maxCount 1;
    ].

:BankEmployeeCorporateTitleMembershipDuration a rdfs:Class, sh:NodeShape;
    rdfs:subClassOf time:Interval;
    rdfs:label "Corporate Title Duration"@en;
    rdfs:comment """A corporate title duration is a period of time that a bank employee has held a corporate title."""@en;
    sh:targetClass :BankEmployeeCorporateTitleMembershipDuration;
    sh:nodeKind sh:IRI;
    sh:property [
        sh:path time:hasBeginning;
        sh:class :xsdDateTimeInstant;
        sh:minCount 1;
        sh:maxCount 1;
    ];
    sh:property [
        sh:path time:hasEnd;
        sh:class :xsdDateTimeInstant;
        sh:minCount 1;
        sh:maxCount 1;
    ].

:xsdDateTimeInstant a rdfs:Class, sh:NodeShape;
    rdfs:subClassOf time:Instant;
    sh:targetClass :xsdDateTimeInstant;
    sh:nodeKind sh:IRI;
    sh:property [
        sh:path time:inXSDDateTime;
        sh:datatype xsd:dateTime;
        sh:minCount 1;
        sh:maxCount 1;
    ].