@prefix bank-org: <http://example.org/bank-org#>.
@prefix bank-id: <http://example.org/bank-id#>.
@prefix sh: <http://www.w3.org/ns/shacl#>.
@prefix rdf: <http://www.w3.org/1999/02/22-rdf-syntax-ns#>.
@prefix rdfs: <http://www.w3.org/2000/01/rdf-schema#>.
@prefix xsd: <http://www.w3.org/2001/XMLSchema#>.
@prefix foaf: <http://xmlns.com/foaf/0.1#>.
@prefix org: <http://www.w3.org/ns/org#>.
@prefix time: <http://www.w3.org/2006/time#>.

############################################################################################################
#
# Bank Specific Properties, over and above the Organization vocabulary
#
############################################################################################################
bank-id:id a rdf:Property, sh:PropertyShape;
    rdfs:range xsd:string;
    rdfs:label "Employee ID"@en;
    rdfs:comment "An employee ID is a unique identifier for a bank employee."@en;
    sh:path bank-id:id;
    sh:datatype xsd:string;
    sh:minCount 1;
    sh:maxCount 1;
    sh:minLength 7;
    sh:maxLength 7.

bank-id:pid a rdf:Property, sh:PropertyShape;
    rdfs:range xsd:string;
    rdfs:label "Employee ID"@en;
    rdfs:comment "An employee ID is a unique identifier for a bank employee."@en;
    sh:path bank-id:pid;
    sh:datatype xsd:string;
    sh:minCount 1;
    sh:maxCount 1;
    sh:minLength 7;
    sh:maxLength 7.

bank-org:bankOrganizationEmployeeCount a rdf:Property, sh:PropertyShape;
    rdfs:label "Employee ID"@en;
    rdfs:comment "An employee ID is a unique identifier for a bank employee."@en;
    sh:path bank-org:bankOrganizationEmployeeCount;
    sh:datatype xsd:number;
    sh:minCount 1;
    sh:maxCount 1.

bank-org:BankCorporateTitle a rdfs:Class;
    rdfs:subClassOf org:Role;
    rdfs:label "Corporate Title"@en;
    rdfs:comment """A corporate title is a role defined by a banking organization that reflects both seniority, but also implies a certain 
                    salary band.  This is in contrast to other types of organization where corporate title and level (pay) are separate."""@en.

bank-org:StaffTitle a bank-org:BankCorporateTitle;
    rdfs:label "Staff"@en;
    rdfs:comment "A staff title is a corporate title that is held by a bank employee."@en.
bank-org:AVPTitle a bank-org:BankCorporateTitle;
    rdfs:label "AVP"@en;
    rdfs:comment "An AVP title is Assistant Vice President corporate title that is held by a bank employee."@en.
bank-org:VPTitle a bank-org:BankCorporateTitle;
    rdfs:label "VP"@en;
    rdfs:comment "A VP title is a Vice President corporate title that is held by a bank employee."@en.
bank-org:SVPTitle a bank-org:BankCorporateTitle;
    rdfs:label "Senior VP"@en;
    rdfs:comment "An VP title is a Senior Vice President corporate title that is held by a bank employee."@en.
bank-org:DIRTitle a bank-org:BankCorporateTitle;
    rdfs:label "Director"@en;
    rdfs:comment "A director title is a corporate title that is held by a bank employee."@en.
bank-org:SDIRTitle a bank-org:BankCorporateTitle;
    rdfs:label "Senior Director"@en;
    rdfs:comment "A SDIR title is a Senior Director corporate title that is held by a bank employee."@en.
bank-org:MDRTitle a bank-org:BankCorporateTitle;
    rdfs:label "Managing Director"@en;
    rdfs:comment "A managing director title is a corporate title that is held by a bank employee."@en.




bank-org:BankEmployee a rdfs:Class, sh:NodeShape;
    rdfs:subClassOf foaf:Person;
    rdfs:label "Bank Employee"@en;
    rdfs:comment """A Bank Employee is a foaf:person who works for a bank, but will also have other properties
                    relating to the Bank such as an employee identifier, a corporate title, and organization."""@en;
    sh:targetClass bank-org:BankEmployee;
    sh:nodeKind sh:IRI;
    sh:property bank-id:id,
                bank-id:pid;
    sh:property [
        sh:path foaf:firstName;
        sh:datatype xsd:string;
        sh:minCount 1;
        sh:maxCount 1;
        sh:minLength 1;
    ];
    sh:property [
        sh:path foaf:surname;
        sh:datatype xsd:string;
        sh:minCount 1;
        sh:maxCount 1;
        sh:minLength 1;
    ].


############################################################################################################
#
# Bank Employee's Corporate Title for defined period of time
#
############################################################################################################
bank-org:BankEmployeeCorporateTitleMembership a rdfs:Class, sh:NodeShape;
    rdfs:subClassOf org:Membership;
    sh:targetClass bank-org:BankEmployeeCorporateTitleMembership;
    sh:nodeKind sh:IRI;
    sh:property [
        sh:path org:member;
        sh:class bank-org:BankEmployee;
        sh:minCount 1;
        sh:maxCount 1;
    ];
    sh:property [
        sh:path bank-org:BankCorporateTitle;
        sh:node bank-org:BankCorporateTitle;
        sh:minCount 1;
        sh:maxCount 1;
        sh:in (bank-org:StaffTitle bank-org:AVPTitle bank-org:VPTitle bank-org:SVPTitle bank-org:DIRTitle bank-org:SDIRTitle bank-org:MDRTitle);
    ];
    sh:property [
        sh:path org:memberDuring;
        sh:class bank-org:MembershipDuration;
        sh:minCount 1;
        sh:maxCount 1;
    ].

bank-org:MembershipDuration a rdfs:Class, sh:NodeShape;
    rdfs:subClassOf time:Interval;
    rdfs:label "Corporate Title Duration"@en;
    rdfs:comment """A corporate title duration is a period of time that a bank employee has held a corporate title."""@en;
    sh:targetClass bank-org:BankEmployeeCorporateTitleMembershipDuration;
    sh:nodeKind sh:IRI;
    sh:property [
        sh:path time:hasBeginning;
        sh:class bank-org:xsdDateTimeInstant;
        sh:minCount 1;
        sh:maxCount 1;
    ];
    sh:property [
        sh:path time:hasEnd;
        sh:class bank-org:xsdDateTimeInstant;
        sh:minCount 1;
        sh:maxCount 1;
    ].

bank-org:xsdDateTimeInstant a rdfs:Class, sh:NodeShape;
    rdfs:subClassOf time:Instant;
    sh:targetClass bank-org:xsdDateTimeInstant;
    sh:nodeKind sh:IRI;
    sh:property [
        sh:path time:inXSDDateTimeStamp;
        sh:datatype xsd:dateTimeStamp;
        sh:minCount 1;
        sh:maxCount 1;
    ].


############################################################################################################
#
# Organization entity
#
############################################################################################################
bank-org:OrganizationalEntity a sh:NodeShape;
    sh:targetClass org:FormalOrganization;
    sh:nodeKind sh:IRI;
    sh:property [
        sh:path org:name;
        sh:datatype xsd:string;
        sh:minCount 1;
        sh:maxCount 1;
        sh:minLength 1;
    ];
    sh:property [
        sh:path org:subOrganizationOf;
        sh:minCount 0;
        sh:maxCount 1;
    ].

############################################################################################################
#
# Bank Employee's organization entity for a defined period of time
#
############################################################################################################
bank-org:BankEmployeeOrganizationalEntityMembership a rdfs:Class, sh:NodeShape;
    rdfs:subClassOf org:Membership;
    sh:targetClass bank-org:BankEmployeeOrganizationalEntityMembership;
    sh:nodeKind sh:IRI;
    sh:property [
        sh:path org:member;
        sh:class bank-org:BankEmployee;
        sh:minCount 1;
        sh:maxCount 1;
    ];
    sh:property [
        sh:path org:organization;
        sh:class org:FormalOrganization;
        sh:minCount 1;
        sh:maxCount 1;
    ];
    sh:property [
        sh:path org:memberDuring;
        sh:class bank-org:MembershipDuration;
        sh:minCount 1;
        sh:maxCount 1;
    ].



############################################################################################################
#
# Employee Count in an organizational entity at a given point in time
#
############################################################################################################
bank-org:BankNumberOfEmployeesInOrg a rdfs:Class, sh:NodeShape;
    rdfs:label "The number of BankEmployees in the given organization."@en;
    rdfs:comment """An organization is defined as a tree structure."""@en;
    sh:targetClass bank-org:BankNumberOfEmployeesInOrg;
    sh:nodeKind sh:IRI;
    sh:property [
        sh:path org:organization;
        sh:class org:FormalOrganization;
        sh:minCount 1;
        sh:maxCount 1;
    ];
    sh:property [
        sh:path time:inXSDDateTime;
        sh:datatype xsd:dateTime;
        sh:minCount 1;
        sh:maxCount 1;
    ];
    sh:property [
        sh:path bank-org:bankOrganizationEmployeeCount;
        sh:datatype xsd:number;
        sh:minCount 1;
        sh:maxCount 1;
    ].